Cleanup & Soundness

Execution.thy
@@ -1,53 +1,68 @@
 theory Execution
-  imports Trace
+  imports Semantics
 begin
 
-section \<open>Execution\<close>
+chapter \<open>Execution Behaviour\<close>
 
-text \<open>
-Given a trace and evaluation property for actions, define the execution of a trace.
-\<close>
-
-locale execution =
+locale execution = semantics +
   fixes eval :: "'a \<Rightarrow> 's rel" 
-  assumes eval_det: "(m,m') \<in> eval \<alpha> \<Longrightarrow> (m,m'') \<in> eval \<alpha> \<Longrightarrow> m' = m''"
 
 context execution
 begin
 
-inductive trace_mem
+section \<open>Transition Definitions\<close>
+
+text \<open>Environment Transition\<close>
+abbreviation etran ("_ -e\<rightarrow> _" [81,81] 80)
+  where "etran P Q \<equiv> (fst P) = (fst Q)"
+
+text \<open>Program Execution Transition\<close>
+abbreviation ctran ("_ -\<alpha>\<rightarrow> _" [81,81] 80)
+  where "ctran P Q \<equiv> (\<exists>\<alpha>. ((fst P) \<mapsto>\<^sub>\<alpha> (fst Q)) \<and> (snd P,snd Q) \<in> eval \<alpha>)"
+
+text \<open>Program Silent Transition\<close>
+abbreviation stran ("_ -s\<rightarrow> _" [81,81] 80)
+  where "stran P Q \<equiv> (((fst P) \<leadsto> (fst Q)) \<and> (snd P) = (snd Q))"
+
+text \<open>Program Transition\<close>
+abbreviation atran ("_ -c\<rightarrow> _" [81,81] 80)
+  where "atran P Q \<equiv> (P -\<alpha>\<rightarrow> Q \<or> P -s\<rightarrow> Q)"
+
+text \<open>Collect of all possible transitions\<close>
+inductive_set transitions
   where 
-    [intro]: "trace_mem m [] m" | 
-    [intro]: "(m'', m) \<in> eval \<alpha> \<Longrightarrow> trace_mem m t m' \<Longrightarrow> trace_mem m'' (\<alpha>#t) m'"
+    one[intro]: "[s] \<in> transitions" |
+    env[intro]: "s -e\<rightarrow> s' \<Longrightarrow> s'#t \<in> transitions \<Longrightarrow> s#s'#t \<in> transitions" |
+    prg[intro]: "s -\<alpha>\<rightarrow> s' \<Longrightarrow> s'#t \<in> transitions \<Longrightarrow> s#s'#t \<in> transitions" |
+    sil[intro]: "s -s\<rightarrow> s' \<Longrightarrow> s'#t \<in> transitions \<Longrightarrow> s#s'#t \<in> transitions"
+inductive_cases transitionsE[elim]: "t \<in> transitions"
 
-definition ev :: "'a Stmt \<Rightarrow> 's \<Rightarrow> 'a Trace \<Rightarrow> 'a Stmt  \<Rightarrow> 's \<Rightarrow> bool"
-  ("\<langle>_,_\<rangle> \<rightarrow>_\<^sup>* \<langle>_,_\<rangle>" [50,40,40] 70)
-  where "\<langle>c,m\<rangle> \<rightarrow>t\<^sup>* \<langle>c',m'\<rangle> \<equiv> trace_mem m t m' \<and> c \<mapsto>t\<^sup>* c'"
+text \<open>Ensure there is no parallelism within a program\<close>
+fun local_only
+  where 
+    "local_only (c\<^sub>1 || c\<^sub>2) = False" |
+    "local_only (c\<^sub>1 ; c\<^sub>2) = (local_only c\<^sub>1 \<and> local_only c\<^sub>2)" |    
+    "local_only (c\<^sub>1 \<sqinter> c\<^sub>2) = (local_only c\<^sub>1 \<and> local_only c\<^sub>2)" |  
+    "local_only (c*) = (local_only c)" |    
+    "local_only _ = True"
 
-lemma trace_mem_det:
-  assumes "trace_mem m t m'" "trace_mem m t m''"
-  shows "m' = m''"
-  using assms
-proof (induct arbitrary: m'')
-  case (1 m)
-  then show ?case by (auto elim: trace_mem.cases)
-next
-  case (2 m''' m \<alpha> t m')
-  hence a: "(m''', m) \<in> eval \<alpha>" "trace_mem m t m'" "\<forall>m''. trace_mem m t m'' \<longrightarrow> m' = m''"
-    by blast+    
-  show ?case using 2(4)
-  proof (cases rule: trace_mem.cases)
-    case (2 m'''')
-    show ?thesis using eval_det[OF 2(1) a(1)] a(3) 2(2) by blast
-  qed
-qed
+section \<open>Predicate Manipulations\<close>
 
-lemma ev_det:
-  assumes "\<langle>c,m\<rangle> \<rightarrow>t\<^sup>* \<langle>c',m'\<rangle>"
-  assumes "\<langle>c,m\<rangle> \<rightarrow>t\<^sup>* \<langle>c'',m''\<rangle>"
-  shows "m'' = m'"
-  using assms trace_mem_det unfolding ev_def
-  by auto
+text \<open>Weakest Precondition, based on evaluation of an instruction\<close>
+definition wp
+  where "wp a P \<equiv> {m. \<forall>m'. (m,m') \<in> eval a \<longrightarrow> m' \<in> P}"
+
+text \<open>Specification Precondition, ensuring an instruction conforms to a relation\<close>
+definition spec
+  where "spec \<alpha> G \<equiv> {m. \<forall>m\<^sub>1. (m,m\<^sub>1) \<in> eval \<alpha> \<longrightarrow> (m,m\<^sub>1) \<in> G}"
+
+text \<open>Compose two state transitions\<close>
+definition comp (infixr "\<otimes>" 60)
+  where "comp a b \<equiv> {(m,m'). \<exists>m''. (m,m'') \<in> a \<and> (m'',m') \<in> b}"
+
+text \<open>Stabilisation of a predicate under an environment step\<close>
+definition st
+  where "st R P \<equiv> {m. \<forall>m'. (m,m') \<in> R\<^sup>* \<longrightarrow> m' \<in> P}"
 
 end
 
