Global_Rules.thy
@@ -1,0 +1,85 @@
+theory Global_Rules
+  imports Local_Rules Interference
+begin
+
+chapter \<open>Global Rules\<close>
+
+locale global_rules = local_rules re fwd eval + interference re fwd eval
+  for eval :: "'a \<Rightarrow> 's rel"
+  and re :: "'a \<Rightarrow> 'a \<Rightarrow> bool" (infix "\<hookleftarrow>" 100)
+  and fwd :: "'a \<Rightarrow> 'a \<Rightarrow> 'a" ("_\<langle>_\<rangle>" [1000,0] 1000)
+
+context global_rules
+begin
+
+section \<open>Global Rules\<close>
+
+text \<open>Establish the rules of the logic, similar to standard Hoare-logic\<close>
+inductive rules :: "'s rel \<Rightarrow> 's rel \<Rightarrow> ('a,'s) ctxs \<Rightarrow> 's set \<Rightarrow> 'a com \<Rightarrow> 's set \<Rightarrow> bool"
+  ("_,_,_ \<turnstile> _ {_} _" [20,0,0,0,20] 20)
+where
+  thread[intro]: "R,G,X \<turnstile>\<^sub>t P { c } Q \<Longrightarrow> inter R G X c \<Longrightarrow> R,G,X \<turnstile> P { c } Q" |
+  par[intro]:    "R\<^sub>1,G\<^sub>1,X \<turnstile> P\<^sub>1 { c\<^sub>1 } Q\<^sub>1 \<Longrightarrow> R\<^sub>2,G\<^sub>2,X \<turnstile> P\<^sub>2 { c\<^sub>2 } Q\<^sub>2 \<Longrightarrow> G\<^sub>2 \<subseteq> R\<^sub>1 \<Longrightarrow> G\<^sub>1 \<subseteq> R\<^sub>2 \<Longrightarrow> 
+                  R\<^sub>1 \<inter> R\<^sub>2,G\<^sub>1 \<union> G\<^sub>2,X \<turnstile> P\<^sub>1 \<inter> P\<^sub>2 { c\<^sub>1 || c\<^sub>2 } (Q\<^sub>1 \<inter> Q\<^sub>2)" |
+  conseq[intro]: "R,G,X \<turnstile> P { c } Q \<Longrightarrow> P' \<subseteq> P \<Longrightarrow> R' \<subseteq> R \<Longrightarrow> G \<subseteq> G' \<Longrightarrow> Q \<subseteq> Q' \<Longrightarrow> 
+                  R',G',X \<turnstile> P' { c } Q'" |
+  frame[intro]:  "R,G,X \<turnstile> P {c} Q \<Longrightarrow> stable R' M \<Longrightarrow> G \<subseteq> R' \<Longrightarrow> R \<inter> R',G,X \<turnstile> P \<inter> M {c} Q \<inter> M"
+
+section \<open>Elimination Rules\<close>
+
+lemma g_parE [elim]:
+  assumes "R,G,X \<turnstile> P { c\<^sub>1 || c\<^sub>2 } Q"
+  obtains R\<^sub>1 G\<^sub>1 P\<^sub>1 Q\<^sub>1 R\<^sub>2 G\<^sub>2 P\<^sub>2 Q\<^sub>2 where 
+    "R\<^sub>1,G\<^sub>1,X \<turnstile> P\<^sub>1 { c\<^sub>1 } Q\<^sub>1" "R\<^sub>2,G\<^sub>2,X \<turnstile> P\<^sub>2 { c\<^sub>2 } Q\<^sub>2"
+    "P \<subseteq> P\<^sub>1 \<inter> P\<^sub>2" "R \<subseteq> R\<^sub>1 \<inter> R\<^sub>2" "G\<^sub>1 \<union> G\<^sub>2 \<subseteq> G" "Q\<^sub>1 \<inter> Q\<^sub>2 \<subseteq> Q" "G\<^sub>1 \<subseteq> R\<^sub>2" "G\<^sub>2 \<subseteq> R\<^sub>1"
+  using assms
+proof (induct R G X P "c\<^sub>1 || c\<^sub>2" Q)
+  case (thread R G X P Q)
+  then show ?case using parE by fast
+next
+  case (par R\<^sub>1 G\<^sub>1 X P\<^sub>1 Q\<^sub>1 R\<^sub>2 G\<^sub>2 P\<^sub>2 Q\<^sub>2)
+  show ?case using par(7)[OF par(1,3)] par(5,6) by blast
+next
+  case (conseq R G X P Q P' R' G' Q')
+  show ?case
+  proof (rule conseq(2), goal_cases)
+    case (1 R\<^sub>1 G\<^sub>1 P\<^sub>1 Q\<^sub>1 R\<^sub>2 G\<^sub>2 P\<^sub>2 Q\<^sub>2)
+    then show ?case using conseq(3,4,5,6) conseq(7)[OF 1(1,2)] by blast
+  qed  
+next
+  case (frame R G X P Q R' M)
+  show ?case
+  proof (rule frame(2), goal_cases)
+    case (1 R\<^sub>1 G\<^sub>1 P\<^sub>1 Q\<^sub>1 R\<^sub>2 G\<^sub>2 P\<^sub>2 Q\<^sub>2)
+    hence a: "R\<^sub>1 \<inter> R',G\<^sub>1,X \<turnstile> P\<^sub>1 \<inter> M {c\<^sub>1} Q\<^sub>1 \<inter> M" "R\<^sub>2 \<inter> R',G\<^sub>2,X \<turnstile> P\<^sub>2 \<inter> M {c\<^sub>2} Q\<^sub>2 \<inter> M"
+      using rules.frame frame(3,4) by auto
+    show ?case using 1(3,4,5,6,7,8) frame(4) frame(5)[OF a] by blast
+  qed
+qed
+
+lemma g_nilE [elim!]:
+  assumes "R,G,X \<turnstile> P {Nil} Q"
+  obtains M where "stable R M" "P \<subseteq> M" "M \<subseteq> Q"
+  using assms by (induct R G X P "Nil :: 'a com" Q) blast+
+
+lemma g_stable_preE:
+  assumes "R,G,X \<turnstile> P {c} Q"
+  obtains P' where "P \<subseteq> P'" "stable R P'" "R,G,X \<turnstile> P' {c} Q"
+  using assms 
+proof (induct)
+  case (thread R G X P c Q)
+  then show ?case using stable_preE by (metis rules.thread) 
+next
+  case (par R\<^sub>1 G\<^sub>1 X P\<^sub>1 c\<^sub>1 Q\<^sub>1 R\<^sub>2 G\<^sub>2 P\<^sub>2 c\<^sub>2 Q\<^sub>2)
+  show ?case
+  proof (rule par(2), rule par(4), goal_cases)
+    case (1 P1 P2)
+    hence "R\<^sub>1 \<inter> R\<^sub>2,G\<^sub>1 \<union> G\<^sub>2,X \<turnstile> P1 \<inter> P2 {c\<^sub>1 || c\<^sub>2} Q\<^sub>1 \<inter> Q\<^sub>2"
+      using rules.par par(5,6) by simp
+    thus ?case using par(7)[of "P1 \<inter> P2"] using 1 by auto
+  qed 
+qed blast+
+
+end
+
+end
