Interference.thy
@@ -1,0 +1,79 @@
+theory Interference
+  imports Execution
+begin
+
+locale interference = execution re fwd eval
+  for re :: "'a \<Rightarrow> 'a \<Rightarrow> bool" (infix "\<hookleftarrow>" 100)
+  and fwd :: "'a \<Rightarrow> 'a \<Rightarrow> 'a" ("_\<langle>_\<rangle>" [1000,0] 1000)
+  and eval :: "'a \<Rightarrow> 's rel"
+
+context interference
+begin
+
+section \<open>Interference Definitions\<close>
+
+text \<open>Independence of two instructions \<beta> and \<alpha> under environment R, 
+      such that the early execution of \<alpha> is assumed to be possible and 
+      cannot invalidate sequential reasoning\<close>
+definition inter\<^sub>a
+  where "inter\<^sub>a R G X \<beta> \<alpha> \<equiv> 
+          (X \<beta> \<inter> wp \<beta> (X \<alpha>) \<subseteq> X \<alpha>\<langle>\<beta>\<rangle> \<inter> wp \<alpha>\<langle>\<beta>\<rangle> (st R (X \<beta>)) \<and> 
+          (eval \<alpha>\<langle>\<beta>\<rangle> \<otimes> R\<^sup>* \<otimes> eval \<beta> \<subseteq> R\<^sup>* \<otimes> eval \<beta> \<otimes> R\<^sup>* \<otimes> eval \<alpha> \<otimes> R\<^sup>*)) \<and>
+          (X \<alpha>\<langle>\<beta>\<rangle> \<subseteq> spec \<alpha>\<langle>\<beta>\<rangle> G)"
+
+text \<open>Independence of program c and instruction \<alpha> under environment R, 
+      such that the early execution of \<alpha> is assumed to be possible and 
+      cannot invalidate sequential reasoning\<close>
+fun inter\<^sub>c
+  where
+    "inter\<^sub>c R G X (Basic \<beta>) \<alpha> = inter\<^sub>a R G X \<beta> \<alpha>" |
+    "inter\<^sub>c R G X (c\<^sub>1 ; c\<^sub>2) \<alpha> = (inter\<^sub>c R G X c\<^sub>1 \<alpha>\<llangle>c\<^sub>2\<rrangle> \<and> inter\<^sub>c R G X c\<^sub>2 \<alpha>)" |
+    "inter\<^sub>c R G X (c\<^sub>1 \<sqinter> c\<^sub>2) \<alpha> = (inter\<^sub>c R G X c\<^sub>1 \<alpha> \<and> inter\<^sub>c R G X c\<^sub>2 \<alpha>)" |
+    "inter\<^sub>c R G X (c*) \<alpha> = inter\<^sub>c R G X c \<alpha>" |
+    "inter\<^sub>c R G X _ \<alpha> = True"
+
+text \<open>Instrumented version of the semantics that collects the reordering effects\<close>
+inductive_set execute_collect :: "('a com \<times> 'a \<times> 'a com \<times> 'a \<times> 'a com) set"
+  and execute_collect_abv :: "'a com \<Rightarrow> 'a \<Rightarrow> 'a com \<Rightarrow> 'a \<Rightarrow> 'a com \<Rightarrow> bool"
+  ("_ \<mapsto>[_,_,_] _" [71,0,0,0,71] 70)
+  where
+  "c \<mapsto>[\<alpha>,t,\<gamma>] c' \<equiv> (c, \<alpha>, t, \<gamma>, c') \<in> execute_collect" |
+  act[intro]:  "Basic \<alpha> \<mapsto>[\<alpha>,Nil,\<alpha>] Nil" |
+  pre[intro]:  "c\<^sub>1 \<mapsto>[\<alpha>,c,\<alpha>'] c\<^sub>1' \<Longrightarrow> c\<^sub>1 ; c\<^sub>2 \<mapsto>[\<alpha>,c,\<alpha>'] c\<^sub>1' ; c\<^sub>2" |
+  pst[intro]:  "c\<^sub>1 \<mapsto>[\<alpha>,c,\<alpha>'] c\<^sub>1' \<Longrightarrow> \<gamma> < c\<^sub>2 <\<^sub>p \<alpha> \<Longrightarrow> c\<^sub>2 ; c\<^sub>1 \<mapsto>[\<gamma>,c\<^sub>2;c,\<alpha>'] c\<^sub>2 ; c\<^sub>1'"
+inductive_cases execute_collect[elim]: "c\<^sub>1 \<mapsto>[\<alpha>,c,\<alpha>'] c\<^sub>1'"
+
+text \<open>Interference property preserved throughout execution\<close>
+inductive inter
+  where "(\<forall>c' \<alpha> \<alpha>' r. c \<mapsto>[\<alpha>,r,\<alpha>'] c' \<longrightarrow> (inter R G X c' \<and> inter\<^sub>c R G X r \<alpha>')) \<Longrightarrow> 
+         (\<forall>c'. c \<leadsto> c' \<longrightarrow> inter R G X c') \<Longrightarrow> inter R G X c"
+
+text \<open>Interference is preserved across a silent step\<close>
+lemma inter_silentI [intro]:
+  assumes "inter R G X c" "c \<leadsto> c'"
+  shows "inter R G X c'"
+  using assms 
+  by cases auto
+
+text \<open>Interference is preserved across an execution step and prevents interference\<close>
+lemma indep_stepI [intro]:
+  assumes "inter R G X c" "c \<mapsto>[\<alpha>,r,\<alpha>'] c'"
+  shows "inter R G X c' \<and> inter\<^sub>c R G X r \<alpha>'"
+  using assms 
+  by cases auto
+
+text \<open>Instrumented semantics collects valid reorderings\<close>
+lemma collect_reorder:
+  assumes "c \<mapsto>[\<alpha>',r,\<alpha>] c'"
+  shows "\<alpha>' < r <\<^sub>p \<alpha>"
+  using assms by (induct, auto)
+
+text \<open>Convert a normal execution step into an instrumented step\<close>
+lemma exec_collect:
+  assumes "c \<mapsto>\<^sub>\<alpha> c'" "local_only c"
+  shows "\<exists>r \<alpha>'. c \<mapsto>[\<alpha>,r,\<alpha>'] c'"
+  using assms by induct auto
+
+end
+
+end
