Soundness.thy
@@ -1,0 +1,350 @@
+theory Soundness
+  imports Global_Rules
+begin
+
+chapter \<open>Soundness\<close>
+
+locale soundness = global_rules
+
+context soundness
+begin
+
+section \<open>Soundness Definitions\<close>
+
+text \<open>Valid transitions starting from a particular program\<close>
+definition cp
+  where "cp c \<equiv> {t. t \<in> transitions \<and> fst (t ! 0) = c}"
+
+text \<open>Traces that satisfy a precondition\<close>
+definition pre
+  where "pre P \<equiv> {t. snd (t!0) \<in> P}"
+
+text \<open>Traces that satisfy a rely\<close>
+definition rely
+  where "rely R \<equiv> {t. (\<forall>i. Suc i < length t \<longrightarrow> t!i -e\<rightarrow> t!Suc i \<longrightarrow> (snd(t!i), snd(t!Suc i)) \<in> R)}"
+
+text \<open>Traces that satisfy a guarantee\<close>
+definition guar
+  where "guar G \<equiv> {t. (\<forall>i. Suc i < length t \<longrightarrow> t!i -c\<rightarrow> t!Suc i \<longrightarrow> (snd(t!i), snd(t!Suc i)) \<in> G\<^sup>=)}"
+
+text \<open>Traces that satisfy a postcondition\<close>
+definition post
+  where "post Q \<equiv> {t. fst (last t) = Nil \<longrightarrow> snd (last t) \<in> Q}"
+
+text \<open>Validity of the rely/guarantee judgements\<close>
+definition validity ("\<Turnstile> _ SAT [_, _, _, _]" [60,0,0,0,0] 45) 
+  where "\<Turnstile> c SAT [P, R, G, Q] \<equiv> cp c \<inter> pre P \<inter> rely R \<subseteq> guar G \<inter> post Q"
+
+text \<open>Strongest postcondition with N environment steps, 
+      used to compute some new intermediate states for reasoning\<close>
+definition sp
+  where "sp a R P \<equiv> {m. \<exists>m' m''. m' \<in> P \<and> (m',m'') \<in> eval a \<and> (m'',m) \<in> R\<^sup>* }"
+
+section \<open>Helper Lemmas\<close>
+
+lemma guar [simp]:
+  "(s # s' # t \<in> guar G) = (s' # t \<in> guar G \<and> (s -c\<rightarrow> s' \<longrightarrow> (snd s, snd s') \<in> G\<^sup>=))"
+  unfolding guar_def using length_Suc_conv less_Suc_eq_0_disj by auto
+
+lemma rely [simp]:
+  "(s # s' # t \<in> rely R) = (s' # t \<in> rely R \<and> (s -e\<rightarrow> s' \<longrightarrow> (snd s, snd s') \<in> R))"
+  unfolding rely_def using length_Suc_conv less_Suc_eq_0_disj by auto
+
+lemma pre [simp]:
+  "(s # t \<in> pre P) = (snd s \<in> P)"
+  by (auto simp: pre_def)
+
+lemma post [simp]:
+  "([x] \<in> post P) = (fst x = Nil \<longrightarrow> snd x \<in> P)"
+  "(s # s' # t \<in> post Q) = (s' # t \<in> post Q)"
+  by (auto simp: post_def)
+
+section \<open>Reordering Rules\<close>
+
+lemma stable_transitive:
+  assumes "(m,m') \<in> R\<^sup>*" "m \<in> P" "stable R P"
+  shows "m' \<in> P"
+  using assms by (induct rule: rtrancl.induct) (auto simp: stable_def)
+
+lemma stable_stI [intro]:
+  assumes "stable R P"
+  shows "P \<subseteq> st R P"
+  using assms stable_transitive by (auto simp: st_def)
+
+lemma atomic_strongest:
+  assumes "R,G,X \<turnstile>\<^sub>A P {\<alpha>} Q"
+  shows "(R,G,X \<turnstile>\<^sub>A P {\<alpha>} (sp \<alpha> R P)) \<and> sp \<alpha> R P \<subseteq> Q"
+proof -
+  have "Q \<subseteq> st R Q" "P \<subseteq> wp \<alpha> Q" 
+    using assms stable_transitive unfolding atomic_rule_def st_def wp_def by fast+
+  hence "sp \<alpha> R P \<subseteq> Q" by (auto simp: sp_def wp_def st_def)
+  moreover have "R,G,X \<turnstile>\<^sub>A P {\<alpha>} (sp \<alpha> R P)"
+    using assms by (clarsimp simp add: atomic_rule_def wp_def stable_def sp_def) force
+  ultimately show ?thesis by auto
+qed
+
+text \<open>
+  Reorder the judgements of two reorderable instructions given a suitable interference property.
+  The precondition P and postcondition Q are preserved.
+\<close>
+lemma reorder_action:
+  assumes "R,G,X \<turnstile>\<^sub>A P {\<beta>} M" "R,G,X \<turnstile>\<^sub>A M {\<alpha>} Q" "\<beta> \<hookleftarrow> fwd \<alpha> \<beta>" "inter\<^sub>a R G X \<beta> \<alpha>"
+  obtains M' where "R,G,X \<turnstile>\<^sub>A P {fwd \<alpha> \<beta>} M'" "R,G,X \<turnstile>\<^sub>A M' {\<beta>} Q"
+proof -
+  \<comment> \<open>Nominate the weakest-precondition of \<beta> over Q as the state between the new \<alpha> and \<beta>\<close>
+  let ?\<alpha>="fwd \<alpha> \<beta>"
+  let ?M="sp ?\<alpha> R P"
+
+  \<comment> \<open>Extract order independence properties\<close>
+  have inter: "X \<beta> \<inter> wp \<beta> (X \<alpha>) \<subseteq> X ?\<alpha> \<inter> wp ?\<alpha> (st R (X \<beta>))"
+    using assms(4) by (auto simp: inter\<^sub>a_def)
+  have "eval ?\<alpha> \<otimes> R\<^sup>* \<otimes> eval \<beta> \<subseteq> R\<^sup>* \<otimes> eval \<beta> \<otimes> R\<^sup>* \<otimes> eval \<alpha> \<otimes> R\<^sup>*"
+    using assms(4) by (auto simp: inter\<^sub>a_def)
+  hence env: "\<forall>Q. st R (wp \<beta> (st R (wp \<alpha> (st R Q)))) \<subseteq> wp ?\<alpha> (st R (wp \<beta> Q))"
+    unfolding comp_def wp_def st_def by safe blast 
+  have g: "X ?\<alpha> \<subseteq> spec ?\<alpha> G" using assms(4) by (auto simp: inter\<^sub>a_def)
+
+  \<comment> \<open>Extract stability for P, Q and the new intermediate state\<close>
+  have stablePQ: "stable R P" "stable R Q" "X \<alpha> \<subseteq> spec \<alpha> G" "X \<beta> \<subseteq> spec \<beta> G"
+    using assms(1,2) by (auto simp: atomic_rule_def)
+  have stableM: "stable R ?M"  unfolding stable_def sp_def by force
+
+  \<comment> \<open>Show transition from P to Q is independent of order\<close>
+  have "P \<subseteq> wp \<beta> M" "M \<subseteq> wp \<alpha> Q" "M \<subseteq> st R M" "P \<subseteq> st R P" "Q \<subseteq> st R Q"
+    using assms(1,2) stable_stI unfolding atomic_rule_def wp_def by auto
+  hence "P \<subseteq> st R (wp \<beta> (st R (wp \<alpha> (st R Q))))" unfolding st_def wp_def by blast
+  hence exec: "P \<subseteq> wp ?\<alpha> (st R (wp \<beta> Q))" using env by blast
+
+  \<comment> \<open>Show the contexts for both operations hold under P\<close>
+  have "P \<subseteq> X \<beta> \<inter> wp \<beta> (X \<alpha>)" using assms(1,2) unfolding atomic_rule_def wp_def by blast
+  hence ctx: "P \<subseteq> X ?\<alpha> \<inter> wp ?\<alpha> (st R (X \<beta>))" using inter by blast
+
+  \<comment> \<open>Establish the late judgement over \<beta>\<close>
+  have "R,G,X \<turnstile>\<^sub>A ?M {\<beta>} Q" 
+  proof (unfold atomic_rule_def, intro conjI Int_greatest)
+    show "?M \<subseteq> wp \<beta> Q" using exec unfolding st_def wp_def sp_def by blast
+  next
+    show "?M \<subseteq> X \<beta>" using ctx unfolding st_def wp_def sp_def by blast
+  qed (insert stablePQ stableM, simp)
+
+  \<comment> \<open>Establish the early judgement over the new \<alpha>\<close>
+  moreover have "R,G,X \<turnstile>\<^sub>A P {?\<alpha>} ?M"
+  proof (unfold atomic_rule_def, intro conjI Int_greatest)
+    show "P \<subseteq> wp ?\<alpha> ?M" unfolding wp_def wf_def sp_def by blast
+  next
+    show "P \<subseteq> X (fwd \<alpha> \<beta>)" using ctx by blast
+  qed (insert stablePQ stableM g, simp)
+
+  ultimately show ?thesis using that by blast
+qed
+
+text \<open>
+  Reorder the judgements of a reorderable instruction \<alpha> and program c, given a suitable 
+  interference property.
+\<close>
+lemma reorder_prog:
+  assumes "R,G,X \<turnstile>\<^sub>t P {c} M" "R,G,X \<turnstile>\<^sub>A M {\<alpha>} Q" "\<alpha>' < c <\<^sub>p \<alpha>" "inter\<^sub>c R G X c \<alpha>"
+  obtains M' P' where "P \<subseteq> P'" "R,G,X \<turnstile>\<^sub>A P' {\<alpha>'} M'" "R,G,X \<turnstile>\<^sub>t M' {c} Q"
+  using assms
+proof (induct c arbitrary: R G X P M Q \<alpha>' \<alpha>)
+  case Nil
+  hence "P \<subseteq> M" by blast
+  then show ?case using Nil by (auto simp: atomic_rule_def)
+next
+  case (Basic \<beta>)
+  have \<alpha>: "\<beta> \<hookleftarrow> \<alpha>\<langle>\<beta>\<rangle>" "\<alpha>' = \<alpha>\<langle>\<beta>\<rangle>" using Basic by auto
+  obtain P' N' where \<beta>: "P \<subseteq> P'" "R,G,X \<turnstile>\<^sub>A P' {\<beta>} N'" "N' \<subseteq> M" using Basic by auto
+  have m': "R,G,X \<turnstile>\<^sub>A N' {\<alpha>} Q"
+    using atomic_pre[OF Basic(3)] \<beta>(2,3) Basic(3) by (auto simp: atomic_rule_def)
+  obtain M' where m'': "R,G,X \<turnstile>\<^sub>A P' {\<alpha>\<langle>\<beta>\<rangle>} M'" "R,G,X \<turnstile>\<^sub>A M' {\<beta>} Q"
+    using reorder_action[OF \<beta>(2) m'(1) \<alpha>(1)] Basic by auto
+  have "R,G,X \<turnstile>\<^sub>t M' {Basic \<beta>} Q" by (rule lrules.basic[OF m''(2)])
+  then show ?case using Basic(1) \<beta>(1) m''(1) \<alpha>(2) by auto
+next
+  case (Seq c\<^sub>1 c\<^sub>2)
+  obtain \<alpha>\<^sub>n where \<alpha>: "\<alpha>' < c\<^sub>1 <\<^sub>p \<alpha>\<^sub>n" "\<alpha>\<^sub>n < c\<^sub>2 <\<^sub>p \<alpha>" using Seq by auto
+  obtain M' where m: "R,G,X \<turnstile>\<^sub>t P {c\<^sub>1} M'" "R,G,X \<turnstile>\<^sub>t M' {c\<^sub>2} M" using Seq(4) by fast
+  have i: "inter\<^sub>c R G X c\<^sub>1 \<alpha>\<^sub>n" "inter\<^sub>c R G X c\<^sub>2 \<alpha>" using Seq \<alpha> by auto
+  show ?case
+  proof (rule Seq(2)[OF _ m(2) Seq(5) \<alpha>(2) i(2)], goal_cases outer)
+    case (outer P' N')
+    hence c1: "R,G,X \<turnstile>\<^sub>t P {c\<^sub>1} P'" using m(1) conseq by auto
+    show ?case 
+    proof (rule Seq(1)[OF _ c1 outer(2) \<alpha>(1) i(1)], goal_cases inner)
+      case (inner P'' M'')
+      then show ?case using Seq(3) outer by auto
+    qed
+  qed
+next
+  case (Choice c\<^sub>1 c\<^sub>2)
+  hence \<alpha>: "\<alpha>' < c\<^sub>1 <\<^sub>p \<alpha>" "\<alpha>' < c\<^sub>2 <\<^sub>p \<alpha>" by auto
+  obtain m: "R,G,X \<turnstile>\<^sub>t P {c\<^sub>1} M" "R,G,X \<turnstile>\<^sub>t P {c\<^sub>2} M" using Choice(4) by blast
+  have i: "inter\<^sub>c R G X c\<^sub>1 \<alpha>" "inter\<^sub>c R G X c\<^sub>2 \<alpha>" using Choice by auto
+  show ?case
+  proof (rule Choice(2)[OF _ m(2) Choice(5) \<alpha>(2) i(2)], goal_cases outer)
+    case (outer P' N')
+    show ?case 
+    proof (rule Choice(1)[OF _ m(1) Choice(5) \<alpha>(1) i (1)], goal_cases inner)
+      case (inner P'' N'')
+      hence "R,G,X \<turnstile>\<^sub>t (N' \<inter> N'') {c\<^sub>1} Q"
+        using outer by (meson Int_lower2 subset_refl lrules.conseq)
+      moreover have "R,G,X \<turnstile>\<^sub>t (N' \<inter> N'') {c\<^sub>2} Q" 
+        using inner outer by (meson Int_lower1 subset_refl lrules.conseq)
+      ultimately have "R,G,X \<turnstile>\<^sub>t (N' \<inter> N'') {c\<^sub>1 \<sqinter> c\<^sub>2} Q" by auto
+      moreover have "P \<subseteq> P' \<inter> P''" using outer inner by auto
+      ultimately show ?case using actomic_conjI[OF outer(2) inner(2)] Choice(3) by blast 
+    qed
+  qed
+next
+  case (Loop c)
+  then obtain I where i: "P \<subseteq> I" "R,G,X \<turnstile>\<^sub>t I {c} I" "stable R I" "I \<subseteq> M" by auto
+  have [simp]: "\<alpha>' = \<alpha>" using Loop by auto
+  have \<alpha>: "\<alpha> < c <\<^sub>p \<alpha>" using Loop by auto
+  have "R,G,X \<turnstile>\<^sub>A I {\<alpha>} Q" using Loop(4) i(3,4) by (meson atomic_pre)
+  hence s: "R,G,X \<turnstile>\<^sub>A I {\<alpha>} (sp \<alpha> R I)" "sp \<alpha> R I \<subseteq> Q" using atomic_strongest by auto
+  have d: "inter\<^sub>c R G X c \<alpha>" using Loop by auto
+
+  show ?case
+  proof (rule Loop(1)[OF _ i(2) s(1) \<alpha> d], goal_cases outer)
+    case (outer P' I')
+    hence "R,G,X \<turnstile>\<^sub>A I {\<alpha>} I'" using i(3) by (meson atomic_pre)
+    hence "sp \<alpha> R I \<subseteq> I'" using atomic_strongest by auto
+    hence "R,G,X \<turnstile>\<^sub>t (sp \<alpha> R I) {c} (sp \<alpha> R I)" using outer(3) lrules.conseq by simp
+    hence "R,G,X \<turnstile>\<^sub>t (sp \<alpha> R I) {c*} (sp \<alpha> R I)" using s(1) by (meson loop atomic_rule_def)
+    hence "R,G,X \<turnstile>\<^sub>t (sp \<alpha> R I) {c*} Q" using s(2) conseq by blast
+    then show ?case using Loop(2)[OF i(1)] s(1) by simp
+  qed
+qed auto
+
+section \<open>Transition Rules\<close>
+
+text \<open>Local judgements are preserved across silent steps\<close>
+lemma rewriteI [intro]:
+  assumes "R,G,X \<turnstile>\<^sub>t P {c} Q"
+  assumes "c \<leadsto> c'"
+  shows "R,G,X \<turnstile>\<^sub>t P {c'} Q"
+  using assms
+proof (induct arbitrary: c' rule: lrules.induct)
+  case (seq R G X P c\<^sub>1 Q c\<^sub>2 M)
+  show ?case using seq(5,1,2,3,4) by cases blast+
+next
+  case (loop R P G X c)
+  thus ?case by cases blast+
+qed auto
+
+text \<open>Global judgements are preserved across silent steps\<close>
+lemma g_rewriteI [intro]:
+  assumes "R,G,X \<turnstile> P {c} Q"
+  assumes "c \<leadsto> c'"
+  shows "R,G,X \<turnstile> P {c'} Q"
+  using assms
+proof (induct arbitrary: c' rule: rules.induct)
+  case (par R\<^sub>1 G\<^sub>1 X P\<^sub>1 c\<^sub>1 Q\<^sub>1 R\<^sub>2 G\<^sub>2 P\<^sub>2 c\<^sub>2 Q\<^sub>2)
+  show ?case using par(7,1,2,3,4,5,6) by cases blast+
+qed auto
+
+text \<open>Local judgements are preserved across execution steps\<close>
+lemma stepI:
+  assumes "c \<mapsto>[\<alpha>,r,\<alpha>'] c'" "R,G,X \<turnstile>\<^sub>t P {c} Q"
+  assumes "inter\<^sub>c R G X r \<alpha>'"
+  shows "\<exists>P' M. P \<subseteq> P' \<and> (R,G,X \<turnstile>\<^sub>A P' {\<alpha>} M) \<and> (R,G,X \<turnstile>\<^sub>t M {c'} Q)"
+  using assms
+proof (induct arbitrary: P R G X Q)
+  case (act \<alpha>)
+  then show ?case by (elim basicE) (meson atomic_rule_def nil lrules.conseq order_refl)
+next
+  case (pre c\<^sub>1 \<alpha> c \<alpha>' c\<^sub>1' c\<^sub>2)
+  obtain M' where m: "R,G,X \<turnstile>\<^sub>t P {c\<^sub>1} M'" "R,G,X \<turnstile>\<^sub>t M' {c\<^sub>2} Q" using pre by fast
+  then show ?case using pre(2)[OF m(1) pre(4)] m(2) by blast
+next
+  case (pst c\<^sub>2 \<alpha> c \<alpha>' c\<^sub>2' \<gamma> c\<^sub>1)
+  obtain M' where m: "R,G,X \<turnstile>\<^sub>t P {c\<^sub>1} M'" "R,G,X \<turnstile>\<^sub>t M' {c\<^sub>2} Q" using pst by fast
+  have i: "inter\<^sub>c R G X c\<^sub>1 (fwd_prog \<alpha>' c)" "inter\<^sub>c R G X c \<alpha>'" using pst by auto
+  obtain P' M where m': "M' \<subseteq> P'" "R,G,X \<turnstile>\<^sub>A P' {\<alpha>} M" "R,G,X \<turnstile>\<^sub>t M {c\<^sub>2'} Q"
+    using pst(2)[OF m(2) i(2)] by blast
+  hence m'': "R,G,X \<turnstile>\<^sub>t P {c\<^sub>1} P'" using m(1) by blast
+  have "fwd_prog \<alpha>' c = \<alpha>" using pst(1) collect_reorder by auto
+  then show ?case using reorder_prog[OF m'' m'(2) pst(3)] i(1) m'(3) by (metis seq)
+qed 
+
+text \<open>Global judgements are preserved across execution steps\<close>
+lemma g_stepI:
+  assumes "R,G,X \<turnstile> P {c} Q"
+  assumes "c \<mapsto>\<^sub>\<alpha> c'"
+  shows "\<exists>P' M. P \<subseteq> P' \<and> (R,G,X \<turnstile>\<^sub>A P' {\<alpha>} M) \<and> (R,G,X \<turnstile> M {c'} Q)"
+  using assms
+proof (induct arbitrary: \<alpha> c' rule: rules.induct)
+  case (par R\<^sub>1 G\<^sub>1 X P\<^sub>1 c\<^sub>1 Q\<^sub>1 R\<^sub>2 G\<^sub>2 P\<^sub>2 c\<^sub>2 Q\<^sub>2)
+  show ?case using par(7)
+  proof cases
+    case (par1 c\<^sub>1')
+    obtain M\<^sub>2 where m2: "P\<^sub>2 \<subseteq> M\<^sub>2" "stable R\<^sub>2 M\<^sub>2" "R\<^sub>2,G\<^sub>2,X \<turnstile> M\<^sub>2 {c\<^sub>2} Q\<^sub>2" using par
+      by (meson g_stable_preE)
+    obtain P M\<^sub>1 where m1: "P\<^sub>1 \<subseteq> P" "R\<^sub>1,G\<^sub>1,X \<turnstile>\<^sub>A P { \<alpha> } M\<^sub>1" "R\<^sub>1,G\<^sub>1,X \<turnstile> M\<^sub>1 {c\<^sub>1'} Q\<^sub>1" 
+      using par1 par(2)[OF par1(2)] by blast
+    hence "R\<^sub>1 \<inter> R\<^sub>2,G\<^sub>1 \<union> G\<^sub>2,X \<turnstile> M\<^sub>1 \<inter> M\<^sub>2 {c'} Q\<^sub>1 \<inter> Q\<^sub>2" using par1 m2 par by blast
+    moreover have "R\<^sub>1 \<inter> R\<^sub>2,G\<^sub>1 \<union> G\<^sub>2,X \<turnstile>\<^sub>A P \<inter> M\<^sub>2 { \<alpha> } M\<^sub>1 \<inter> M\<^sub>2" 
+      using m1(2) m2(2) par.hyps(6) by blast
+    ultimately show ?thesis using m2(1) m1(1) by blast
+  next
+    case (par2 c\<^sub>2')
+    obtain M\<^sub>1 where m1: "P\<^sub>1 \<subseteq> M\<^sub>1" "stable R\<^sub>1 M\<^sub>1" "R\<^sub>1,G\<^sub>1,X \<turnstile> M\<^sub>1 {c\<^sub>1} Q\<^sub>1" using par
+      by (meson g_stable_preE)
+    obtain P M\<^sub>2 where m2: "P\<^sub>2 \<subseteq> P" "R\<^sub>2,G\<^sub>2,X \<turnstile>\<^sub>A P { \<alpha> } M\<^sub>2" "R\<^sub>2,G\<^sub>2,X \<turnstile> M\<^sub>2 {c\<^sub>2'} Q\<^sub>2"
+      using par2 par(4)[OF par2(2)] by blast
+    hence "R\<^sub>1 \<inter> R\<^sub>2,G\<^sub>1 \<union> G\<^sub>2,X \<turnstile> M\<^sub>1 \<inter> M\<^sub>2 {c'} Q\<^sub>1 \<inter> Q\<^sub>2" using par2 m1 par by blast
+    moreover have "R\<^sub>2 \<inter> R\<^sub>1,G\<^sub>1 \<union> G\<^sub>2,X \<turnstile>\<^sub>A P \<inter> M\<^sub>1 { \<alpha> } M\<^sub>2 \<inter> M\<^sub>1" 
+      using atomic_frameI[OF m2(2) m1(2) par(5)] by blast
+    ultimately show ?thesis using m2(1) m1(1) by (metis inf_commute inf_mono)
+  qed 
+next
+  case (conseq R G X P c Q P' R' G' Q')
+  thus ?case using rules.conseq atomic_conseqI by (meson order_refl subset_trans)
+next
+  case (frame R G X P c Q R' M')
+  then obtain P' M where "P \<subseteq> P'" "R,G,X \<turnstile>\<^sub>A P' {\<alpha>} M" "R,G,X \<turnstile> M {c'} Q" by metis
+  thus ?case using rules.frame atomic_frameI frame(3,4) by blast
+next
+  case (thread R G X P c Q)
+  hence "local_only c" using thread_only by auto
+  then obtain r \<alpha>'' where c: "c \<mapsto>[\<alpha>,r,\<alpha>''] c'" using thread exec_collect by blast
+  then show ?case 
+    using stepI[OF c thread(1)] thread(2) indep_stepI[OF thread(2) c] by auto 
+qed
+
+section \<open>Theorem\<close>
+
+text \<open>All transitions that start with a program with a logic judgement and satisfy
+      the precondition and environment rely should conform to the guarantee and
+      establish the postcondition if they terminate\<close>
+lemma sound_transitions:
+  assumes "t \<in> transitions" "fst (t ! 0) = c" "R,G,X \<turnstile> P {c} Q" "t \<in> pre P \<inter> rely R"
+  shows "t \<in> guar G \<inter> post Q"
+  using assms
+proof (induct arbitrary: c P rule: transitions.induct)
+  case (one s)
+  thus ?case using guar_def by force
+next
+  case (env s s' t)
+  then obtain P' where "P \<subseteq> P'" "stable R P'" "R,G,X \<turnstile> P' {c} Q" by (metis g_stable_preE) 
+  thus ?case using env by (auto simp: stable_def)
+next
+  case (prg s s' t)
+  then obtain \<alpha> where \<alpha>: "c \<mapsto>\<^sub>\<alpha> (fst s')" "(snd s,snd s') \<in> eval \<alpha>" by auto
+  then obtain P' M where "P \<subseteq> P'" "R,G,X \<turnstile>\<^sub>A P' {\<alpha>} M" "R,G,X \<turnstile> M {fst s'} Q"
+    using g_stepI[OF prg(5) \<alpha>(1)] by metis
+  thus ?case using prg \<alpha> unfolding atomic_rule_def wp_def spec_def by fastforce
+next
+  case (sil s s' t)
+  thus ?case by auto
+qed
+
+text \<open>Soundness Theorem\<close>
+theorem sound:
+  assumes "R,G,X \<turnstile> P { c } Q"
+  shows "\<Turnstile> c SAT [P, R, G, Q]"
+  using assms sound_transitions by (auto simp: validity_def cp_def)
+
+end
+
+end
