README.md
@@ -2,3 +2,20 @@
 
 This project contains the Isabelle/HOL formalisation and soundness proof for a rely/guarantee logic tailored to weak memory
 models based on a notion of interfering local operation pairs.
+
+## Layout
+- Semantics.thy: Weak memory small step semantics, based on Rob's reordering + forwarding
+- Execution.thy: Couple semantics with evaluation of instructions and arbitrary environment steps
+- Interference.thy: Abstract definition the thread-local interference analysis
+- Local_Rules.thy: Thread-local rely/guarantee reasoning
+- Global_Rules.thy: Parallel composition of thread-local reasoning
+- Soundness.thy: Definition and proof of soundness
+
+## TODO
+- [ ] Specialise semantics for ARMv8
+- [ ] Finish verification of executable interference analysis
+- [ ] Add WP + verify some examples using Nieto's automation
+- [ ] State dependent reordering
+- [ ] NMCA semantics + interference analysis
+- [ ] Explore moving interference to sequential composition
+- [ ] Explore completeness issues
